Algorithm/Data/Classes/MinHeap.lean
@@ -16,23 +16,25 @@ theorem inf_eq_top {m : Multiset α} : m.inf = ⊤ ↔ ∀ a ∈ m, a = ⊤ := b
 
 end Multiset
 
-class MinHeap (C : Type*) (α : outParam Type*) [LinearOrder α] extends
+class MinHeap (C : Type*) (α : outParam Type*)
+    [Preorder α] [IsTotalPreorder α (· ≤ ·)] extends
     ToMultiset C α,
     EmptyCollection C, ToMultiset.LawfulEmptyCollection C α,
     Insert α C, ToMultiset.LawfulInsert C α where
   head? : C → WithTop α
-  head?_def c : head? c = ((toMultiset c).map WithTop.some).inf
+  head?_eq_top c : isEmpty c → head? c = ⊤
+  head?_mem_toMultiset_map c : ¬isEmpty c → (head? c) ∈ (toMultiset c).map (↑)
+  head?_le (c : C) : ∀ x ∈ c, head? c ≤ x
   headD : C → α → α :=
     fun s d ↦ (head? s).getD d
   head (c : C) : ¬isEmpty c → α :=
-    fun h ↦ (head? c).untop fun hc ↦ h (by
-      rw [isEmpty_iff_size_eq_zero, size_eq_card_toMultiset, Multiset.card_eq_zero,
-        Multiset.eq_zero_iff_forall_not_mem]
-      simpa [head?_def] using hc)
+    fun h ↦ (head? c).untop fun hc ↦ by
+      have := hc ▸ (head?_mem_toMultiset_map c h)
+      simp at this
   headD_def c d : headD c d = (head? c).getD d := by intros; rfl
-  head_eq_head? c h : head c h = head? c := by simp
+  coe_head_eq_head? c h : head c h = head? c := by simp
   tail : C → C
-  toMultiset_tail c : toMultiset (tail c) =
+  toMultiset_tail c : [DecidableEq α] → toMultiset (tail c) =
     if h : isEmpty c then 0 else (toMultiset c).erase (head c h)
   deleteMin : C → Option (α × C) := fun c ↦ if h : isEmpty c then none else
     some (head c h, tail c)
@@ -41,19 +43,66 @@ class MinHeap (C : Type*) (α : outParam Type*) [LinearOrder α] extends
 
 namespace MinHeap
 
-attribute [simp] head?_def headD_def toMultiset_tail deleteMin_def
+attribute [simp] headD_def toMultiset_tail deleteMin_def
 
-variable {C α : Type*} [LinearOrder α] [MinHeap C α] {c : C}
+section
+
+variable {C α : Type*} [Preorder α] [IsTotalPreorder α (· ≤ ·)] [MinHeap C α] (c : C)
 
 lemma head?_ne_top (h : ¬isEmpty c) :
-    (MinHeap.head? c) ≠ ⊤ := fun hc ↦ h (by
-  rw [isEmpty_iff_size_eq_zero, size_eq_card_toMultiset, Multiset.card_eq_zero,
-    Multiset.eq_zero_iff_forall_not_mem]
-  simpa [head?_def] using hc)
+    (MinHeap.head? c) ≠ ⊤ := by
+  intro hc
+  have := hc ▸ (head?_mem_toMultiset_map c h)
+  simp at this
 
 @[simp]
 lemma head_def (h : ¬isEmpty c) :
-    MinHeap.head c h = (head? c).untop (head?_ne_top h) :=
-  WithTop.coe_injective (by simpa using MinHeap.head_eq_head? c h)
+    MinHeap.head c h = (head? c).untop (head?_ne_top c h) :=
+  WithTop.coe_injective (by simpa using MinHeap.coe_head_eq_head? c h)
+
+lemma head_mem_toMultiset (h : ¬isEmpty c) :
+    head c h ∈ toMultiset c := by
+  obtain ⟨x, hx₁, hx₂⟩ := Multiset.mem_map.mp (head?_mem_toMultiset_map c h)
+  simp [hx₁, ← hx₂]
+
+lemma head_mem (h : ¬isEmpty c) :
+    head c h ∈ c := by
+  exact mem_toMultiset.mp (head_mem_toMultiset c h)
+
+lemma head_le (x) (hx : x ∈ c) :
+    head c (ToMultiset.not_isEmpty_of_mem hx) ≤ x := by
+  simpa [WithTop.untop_le_iff] using head?_le c x hx
+
+lemma coe_eq_head?_of_forall_le (p : α → Prop) (hc : ¬isEmpty c) (pc : p (head c hc))
+    (x : α) (hx : x ∈ c) (h : ∀ y ∈ c, p y → y ≠ x → x < y) :
+    x = head? c := by
+  contrapose! h
+  exact ⟨head c (ToMultiset.not_isEmpty_of_mem hx), MinHeap.head_mem _ _, pc, by intro h'; simp [← h'] at h,
+    fun h' ↦ (h'.trans_le (head_le c _ hx)).ne rfl⟩
+
+lemma eq_head_of_forall_le (p : α → Prop) (hc : ¬isEmpty c) (pc : p (head c hc))
+    (x : α) (hx : x ∈ c) (h : ∀ y ∈ c, p y → y ≠ x → x < y) :
+    x = head c hc := by
+  apply WithTop.coe_injective
+  simpa using coe_eq_head?_of_forall_le c p hc pc x hx h
+
+end
+
+section LinearOrder
+
+variable {C α : Type*} [LinearOrder α] [MinHeap C α] {c : C}
+
+@[simp]
+lemma head?_def : head? c = ((toMultiset c).map WithTop.some).inf := by
+  by_cases hc : isEmpty c
+  · simp [head?_eq_top c hc, hc]
+  · apply le_antisymm
+    · have := head?_le c
+      aesop
+    · have := head?_mem_toMultiset_map c hc
+      apply Multiset.inf_le
+      aesop
+
+end LinearOrder
 
 end MinHeap
